Prove zero block is a valid inode

src/program_proof/examples/inode_proof.v
@@ -27,8 +27,8 @@ Implicit Types (σ: inode.t).
 Implicit Types (l:loc) (γ:gname) (P: inode.t → iProp Σ).
 
 Definition inode_linv (l:loc) σ : iProp Σ :=
-  ∃ (addr_s: Slice.t) (addrs: list u64) (hdr: Block),
-    "%Hencoded" ∷ ⌜Block_to_vals hdr = b2val <$> encode ([EncUInt64 (U64 $ length addrs)] ++ (map EncUInt64 addrs))⌝ ∗
+  ∃ (addr_s: Slice.t) (addrs: list u64) (extra: list u8) (hdr: Block),
+    "%Hencoded" ∷ ⌜Block_to_vals hdr = b2val <$> encode ([EncUInt64 (U64 $ length addrs)] ++ (map EncUInt64 addrs)) ++ extra⌝ ∗
     "Hhdr" ∷ int.val σ.(inode.addr) d↦ hdr ∗
     "addr" ∷ l ↦[inode.S :: "addr"] #σ.(inode.addr) ∗
     "addrs" ∷ l ↦[inode.S :: "addrs"] (slice_val addr_s) ∗
@@ -45,19 +45,53 @@ Definition is_inode l γ P : iProp Σ :=
                          "Hlock" ∷ is_lock inodeN γ #lref (∃ σ, inode_linv l σ ∗ P σ).
 
 Definition is_inode_durable σ : iProp Σ :=
-  ∃ (addrs: list u64) (hdr: Block),
-    "%Hencoded" ∷ ⌜Block_to_vals hdr = b2val <$> encode ([EncUInt64 (U64 $ length addrs)] ++ (map EncUInt64 addrs))⌝ ∗
+  ∃ (addrs: list u64) (extra: list u8) (hdr: Block),
+    "%Hencoded" ∷ ⌜Block_to_vals hdr = b2val <$> encode ([EncUInt64 (U64 $ length addrs)] ++ (map EncUInt64 addrs)) ++ extra⌝ ∗
     "Hhdr" ∷ int.val σ.(inode.addr) d↦ hdr ∗
     "Hdata" ∷ [∗ list] a;b ∈ addrs;σ.(inode.blocks), int.val a d↦ b.
 
-Theorem is_inode_crash l σ :
+Instance is_inode_crash l σ :
   IntoCrash (inode_linv l σ) (λ _, is_inode_durable σ).
 Proof.
   hnf; iIntros "Hinv".
   iNamed "Hinv".
-  iExists addrs, hdr.
+  iExists addrs, extra, hdr.
   iFrame "% ∗".
   auto.
 Qed.
+
+(* TODO: these are copied from the circ proof *)
+
+Definition block0: Block :=
+  list_to_vec (replicate (Z.to_nat 4096) (U8 0)).
+
+Lemma replicate_zero_to_block0 :
+  replicate (int.nat 4096) (zero_val byteT) =
+  Block_to_vals block0.
+Proof.
+  change (zero_val byteT) with #(U8 0).
+  change (int.nat 4096) with (Z.to_nat 4096).
+  rewrite /Block_to_vals /block0.
+  reflexivity.
+Qed.
+
+Theorem init_inode addr :
+  int.val addr d↦ block0 -∗ is_inode_durable (inode.mk addr []).
+Proof.
+  iIntros "Hhdr".
+  iExists [], (replicate (int.nat (4096-8)) (U8 0)), block0.
+  cbv [inode.addr inode.blocks big_sepL2].
+  iFrame "Hhdr".
+  iPureIntro.
+  reflexivity.
+Qed.
+
+Theorem wp_openInode d addr σ P :
+  addr = σ.(inode.addr) ->
+  {{{ is_inode_durable σ ∗ P σ }}}
+    openInode d #addr
+  {{{ l γ, RET #l; is_inode l γ P }}}.
+Proof.
+Admitted.
 
 End goose.
